\section{Question 3}
Equation of motion:

% \begin{rcases}
%     T_{Dx} = I_x \ddot{\phi} + 4\omega_0^2\left(I_y-I_z\right)\phi- \omega_0\left(I_x + I_y - I_z\right) \dot \psi \\
%     T_{Dz} = I_z \ddot{\psi} + \omega_0^2\left(I_z+I_x-I_y\right)\dot \phi+ \omega_0^2\left(I_y - I_x\right) \psi
%     \end{rcases}\to s^4 + \omega_0^2 \left(3\sigma_x + \sigma_x\sigma_z +1\right)s^2+4\omega_0^2\sigma_x \sigma_z = 0
% $$
% where:
\begin{equation*}
    \begin{split}
    T_{Dx} = I_x \ddot{\phi} + 4\omega_0^2\left(I_y-I_z\right)\phi- \omega_0\left(I_x + I_y - I_z\right) \dot \psi \xrightarrow{\mathscr{L}}
    4\,\phi \,{\left(I_y -I_z \right)}\,{\omega_0 }^2 -\psi \,{\left(I_x +I_y -I_z \right)}\,\omega_0 \,s+I_x \,\phi \,s^2 =0
    \\
    T_{Dz} = I_z \ddot{\psi} + \omega_0^2\left(I_z+I_x-I_y\right)\dot \phi+ \omega_0^2\left(I_y - I_x\right) \psi \xrightarrow{\mathscr{L}} \phi \,{\left(I_x -I_y +I_z \right)}\,{\omega_0 }^2 \,s-\psi \,{\left(I_x -I_y \right)}\,{\omega_0 }^2 +I_z \,\psi \,s^2 =0
    \end{split}
\end{equation*}

Using below terms to simplify the equations.

$$
\sigma_x = \dfrac{I_y-I_z}{I_x}, \quad \sigma_z = \dfrac{I_y-I_x}{I_z}
$$

\begin{equation}
    \begin{split}
        4\,\phi \,\sigma_x \,{\omega_0 }^2 -\psi \,{\left(1-\sigma_x \right)}\,\omega_0 \,s+\phi \,s^2 =0\to \phi [s^2+4\sigma_x\omega_0^2] + \psi[-\omega_0s(1-\sigma_x)] = 0\\
        -\phi \,{\left(\sigma_z -1\right)}\,{\omega_0 }^2 \,s-\psi \,\sigma_z \,{\omega_0 }^2 +\psi \,s^2 =0\to \phi[\omega_0s(1-\sigma_z)]+ \psi[s^2+\omega_0^2\sigma_z] = 0
    \end{split}
\end{equation}

\begin{eqnarray*}
    \begin{bmatrix}
        s^2+4\sigma_x\omega_0^2 & -\omega_0s(1-\sigma_x)\\
        \omega_0s(1-\sigma_z) & s^2+\omega_0^2\sigma_z
    \end{bmatrix}\begin{bmatrix}
        \phi\\
        \psi
    \end{bmatrix} = \boldsymbol{\mathrm{A}} \begin{bmatrix}
        \phi\\
        \psi
    \end{bmatrix} = \begin{bmatrix}
        0\\0
    \end{bmatrix}
\end{eqnarray*}

To avoid the trivial solution ($\phi = \psi = 0$), the determinant of the coefficient matrix must be zero.

\begin{equation*}
    \begin{split}
        \det \boldsymbol{\mathrm{A}} &= {\omega_0 }^2 \,s^2 +s^4 +4\,{\omega_0 }^4 \,\sigma_x \,\sigma_z +3\,{\omega_0 }^2 \,s^2 \,\sigma_x +{\omega_0 }^2 \,s^2 \,\sigma_x \,\sigma_z \\&= s^4   + \omega_0^2(3s^2\sigma_x + \sigma_x\sigma_y + 1)  +4\,{\omega_0 }^4 \,\sigma_x \,\sigma_z = 0
    \end{split}
\end{equation*}